checkpoint

src/cddl/test/dpe/CDDLTest.DPEMain.fst
@@ -15,9 +15,8 @@ module U32 = FStar.UInt32
 #lang-pulse
 
 module I = CDDLTest.DPE.InitializeContextInput
-// module DC = CDDLTest.DPE.DeriveContextInput
-// module SI = CDDLTest.DPE.SignInput
-module CK = CDDLTest.DPE.CertifyKeyInput
+module DC = CDDLTest.DPE.DeriveContextInput
+module CKO = CDDLTest.DPE.CertifyKeyOutput
 open CDDL.Pulse.Types
 open FStar.Seq
 open DPESlice
@@ -86,7 +85,226 @@ ensures (
   }
 }
 
-module CKO = CDDLTest.DPE.CertifyKeyOutput
+let trace_valid_for_derive_context (t:trace) : prop =
+  match current_state t with
+  | G_Available (Engine_context_spec _)
+  | G_Available (L0_context_spec _) -> True
+  | _ -> False
+
+type derive_context_result =
+  | Input_parsing_failure
+  | Missing_arguments
+  | Incorrect_state
+  | Session_error
+  | Success
+
+ghost
+fn is_record_opt_cases e s k
+requires DC.is_record_opt e s k
+ensures  DC.is_record_opt e s k ** pure (Some? e <==> Some? s)
+{
+  admit()
+}
+
+ghost
+fn elim_is_record_opt_none (s:option spec_record_t) k
+requires DC.is_record_opt None s k
+ensures pure (s == None) ** k
+{
+  admit()
+}
+
+ghost
+fn elim_is_record_opt_some (r:record_t) (s:option spec_record_t) k
+requires DC.is_record_opt (Some r) s k
+returns _:squash (Some? s)
+ensures DC.is_derive_context_input_args_data r (Some?.v s) k
+{
+  admit()
+}
+
+
+ghost
+fn claim_is_record_opt (e:option record_t) (s:option spec_record_t) k
+requires DC.is_record_opt e s k
+ensures k
+{
+  admit()
+}
+
+ghost
+fn claim_is_dci (e:record_t) (s:spec_record_t) k
+requires DC.is_derive_context_input_args_data e s k
+ensures k
+{
+  admit()
+}
+
+ghost
+fn is_dci_cases
+    (e:record_t)
+    (res:spec_record_t)
+    (k:slprop)
+requires DC.is_derive_context_input_args_data e res k
+ensures DC.is_derive_context_input_args_data e res k **
+        pure (Inl? e <==> Inl? res)
+{
+  admit()
+}
+
+let current_state_is_l0 (t:trace {trace_valid_for_derive_context t}) : prop =
+  match current_state t with
+  | G_Available (L0_context_spec _) -> True
+  | G_Available (Engine_context_spec _) -> False
+
+fn check_state_l0
+  (sid:sid_t)
+  (#t:G.erased trace { trace_valid_for_derive_context t })
+requires
+  sid_pts_to trace_ref sid t
+returns ok:bool
+ensures
+  sid_pts_to trace_ref sid t
+ensures pure (ok <==> current_state_is_l0 t)
+{
+  admit()
+}
+
+let trace_and_record_invalid_engine
+    (t:trace {trace_valid_for_derive_context t})
+    (e:spec_record_t)
+: Lemma 
+  (requires current_state_is_l0 t /\ Inl? e)
+  (ensures ~(trace_and_record_valid_for_derive_child t e))
+= ()
+
+[@@pulse_unfold]
+let derive_context_post 
+  (sid:sid_t)
+  (t:G.erased trace { trace_valid_for_derive_context t })
+  (p:perm)
+  (w:erased _)
+  (input:Slice.slice U8.t)
+  (res:derive_context_result)
+: slprop
+= match res with
+  | Input_parsing_failure ->
+    sid_pts_to trace_ref sid t
+  | Missing_arguments -> 
+    sid_pts_to trace_ref sid t **
+    pure (DC.is_input_args_data w None)
+  | Incorrect_state ->
+    sid_pts_to trace_ref sid t **
+    pure (exists (spec_record:DPESlice.spec_record_t).
+              {:pattern (DC.is_input_args_data w (Some spec_record))}
+            DC.is_input_args_data w (Some spec_record) /\
+            ~(trace_and_record_valid_for_derive_child t spec_record))
+  | _ -> 
+    exists* (spec_record:DPESlice.spec_record_t).
+        pure (DC.is_input_args_data w (Some spec_record) /\
+              trace_and_record_valid_for_derive_child t spec_record) **
+        derive_child_client_perm sid t spec_record (Success? res)
+
+#push-options "--query_stats"
+
+ghost
+fn take_record_perm 
+  (record:record_t)
+  (spec:spec_record_t)
+  (k:slprop)
+requires DC.is_derive_context_input_args_data record spec k
+ensures record_perm record spec ** Trade.trade (record_perm record spec) k
+{ 
+  admit() //  Trade.Util.rewrite_with_trade k (record_perm record spec);
+}
+
+fn derive_context_aux
+  (sid:sid_t)
+  (#t:G.erased trace)
+  (#p:perm)
+  (#w:erased _)
+  (input:Slice.slice U8.t)
+  (record:record_t)
+  (#spec:erased spec_record_t { trace_and_record_valid_for_derive_child t spec })
+requires
+  DC.is_derive_context_input_args_data record spec (pts_to input #p w) **
+  sid_pts_to trace_ref sid t **
+  pure (DC.is_input_args_data w (Some #spec_record_t spec))
+returns res:derive_context_result
+ensures pts_to input #p w
+ensures derive_context_post sid t p w input res
+{
+  take_record_perm _ _ _;
+  let res = derive_child sid t record;
+  Trade.elim_trade _ _;
+  match res {
+    true -> { Success }
+    false -> { Session_error }
+  }
+}
+
+fn derive_context
+  (sid:sid_t)
+  (#t:G.erased trace { trace_valid_for_derive_context t })
+  (#p:perm)
+  (#w:erased _)
+  (input:Slice.slice U8.t)
+requires
+  pts_to input #p w **
+  sid_pts_to trace_ref sid t
+returns res:derive_context_result
+ensures pts_to input #p w
+ensures derive_context_post sid t p w input res
+{
+  let record_opt, ok = DC.parse_derive_context_input_args input;
+  match ok {
+    false -> {
+      Input_parsing_failure
+    }
+
+    true -> {
+      is_record_opt_cases _ _ _;
+      match record_opt {
+        None -> {
+          elim_is_record_opt_none _ _;
+          Missing_arguments
+        }
+
+        Some record -> {
+          elim_is_record_opt_some _ _ _;
+          is_dci_cases _ _ _;
+          let is_l0 = check_state_l0 sid;
+          if is_l0
+          {
+            match record {
+              Inl _ -> {
+                claim_is_dci _ _ _;
+                Incorrect_state
+              }
+
+              Inr l0 -> {
+                derive_context_aux sid #t #p #w input (Inr l0);
+              }
+            }
+          }
+          else
+          {
+            match record {
+              Inl eng -> {
+                derive_context_aux sid #t #p #w input (Inl eng)
+              }
+
+              Inr l0 -> {
+                claim_is_dci _ _ _;
+                Incorrect_state
+              }
+            }
+          }
+        }
+      }
+    }
+  }
+}
 
 assume
 val max_cert_len : SZ.t
